Rename value -> result

src/PlutusIR/Semantics/Dynamic/Values.v
@@ -14,6 +14,7 @@ Inductive is_error : term -> Prop :=
   | IsError : forall T,
       is_error (Error T).
 
+
 Inductive value : term -> Prop :=
   | V_LamAbs : forall x T t0,
       value (LamAbs x T t0)
@@ -21,18 +22,13 @@ Inductive value : term -> Prop :=
       value (TyAbs X K t)
   | V_IWrap : forall F T v,
       value v ->
-      ~ is_error v ->
       value (IWrap F T v)
   | V_Constant : forall u,
       value (Constant u)
-  | V_Error : forall T,
-      value (Error T)
   | V_Constr : forall i T vs,
       Forall value vs ->
       value (Constr i T vs)
   .
-
-#[export] Hint Constructors value : core.
 
 Section value_ind.
 Context
@@ -41,9 +37,8 @@ Context
 Context
   (H_LamAbs : forall (x : String.string) (T : ty) (t0 : term), P (LamAbs x T t0))
   (H_TyAbs : forall (X : String.string) (K : kind) (t : term), P (TyAbs X K t))
-  (H_IWrap : forall (F T : ty) (v : term), value v -> P v -> ~ is_error v -> P (IWrap F T v))
+  (H_IWrap : forall (F T : ty) (v : term), value v -> P v -> P (IWrap F T v))
   (H_Constant : forall c : constant, P (Constant c))
-  (H_Error : forall T : ty, P (Error T))
   (H_Constr : forall (i : nat) (T : ty) (vs : list term), Forall value vs -> Forall P vs -> P (Constr i T vs))
 .
 Fixpoint values__ind (H_value : forall (t : term), value t -> P t) (ts : list term) (vs : Forall value ts): Forall P ts :=
@@ -55,9 +50,8 @@ Fixpoint value__ind (t : term) (v : value t) {struct v} : P t :=
   match v in (value t0) return (P t0) with
   | V_LamAbs x T t0 => H_LamAbs x T t0
   | V_TyAbs X K t0 => H_TyAbs X K t0
-  | V_IWrap F1 T v0 v1 n => H_IWrap F1 T v0 v1 (value__ind v0 v1) n
+  | V_IWrap F1 T v0 v1 => H_IWrap F1 T v0 v1 (value__ind v0 v1)
   | V_Constant u => H_Constant u
-  | V_Error T => H_Error T
   | V_Constr i T ts vs => H_Constr i T ts vs
       ((fix F ts vs := match vs as vs in Forall _ ts return Forall P ts with
         | Forall_nil _ => Forall_nil _
@@ -67,6 +61,81 @@ Fixpoint value__ind (t : term) (v : value t) {struct v} : P t :=
 .
 
 End value_ind.
+
+
+Inductive result : term -> Prop :=
+  | R_LamAbs : forall x T t0,
+      result (LamAbs x T t0)
+  | R_TyAbs : forall X K t,
+      result (TyAbs X K t)
+  | R_IWrap : forall F T v,
+      result v ->
+      ~ is_error v ->
+      result (IWrap F T v)
+  | R_Constant : forall u,
+      result (Constant u)
+  | R_Error : forall T,
+      result (Error T)
+  | R_Constr : forall i T vs,
+      Forall result vs ->
+      result (Constr i T vs)
+  .
+
+#[export] Hint Constructors result : core.
+
+Section result_ind.
+Context
+  (P : term -> Prop)
+.
+Context
+  (H_LamAbs : forall (x : String.string) (T : ty) (t0 : term), P (LamAbs x T t0))
+  (H_TyAbs : forall (X : String.string) (K : kind) (t : term), P (TyAbs X K t))
+  (H_IWrap : forall (F T : ty) (v : term), result v -> P v -> ~ is_error v -> P (IWrap F T v))
+  (H_Constant : forall c : constant, P (Constant c))
+  (H_Error : forall T : ty, P (Error T))
+  (H_Constr : forall (i : nat) (T : ty) (vs : list term), Forall result vs -> Forall P vs -> P (Constr i T vs))
+.
+Fixpoint results__ind (H_result : forall (t : term), result t -> P t) (ts : list term) (vs : Forall result ts): Forall P ts :=
+  match vs as vs in Forall _ ts return Forall P ts with
+    | Forall_nil _ => Forall_nil _
+    | @Forall_cons _ _ x xs vx vxs => @Forall_cons _ _ x xs (H_result x vx) (results__ind H_result xs vxs)
+  end.
+Fixpoint result__ind (t : term) (v : result t) {struct v} : P t :=
+  match v in (result t0) return (P t0) with
+  | R_LamAbs x T t0 => H_LamAbs x T t0
+  | R_TyAbs X K t0 => H_TyAbs X K t0
+  | R_IWrap F1 T v0 v1 n => H_IWrap F1 T v0 v1 (result__ind v0 v1) n
+  | R_Constant u => H_Constant u
+  | R_Error T => H_Error T
+  | R_Constr i T ts vs => H_Constr i T ts vs
+      ((fix F ts vs := match vs as vs in Forall _ ts return Forall P ts with
+        | Forall_nil _ => Forall_nil _
+        | @Forall_cons _ _ t ts vt vts => @Forall_cons _ _ t ts (result__ind t vt) (F ts vts)
+      end) ts vs)
+  end
+.
+
+End result_ind.
+
+
+Lemma value__is_error v : value v -> ~ is_error v.
+Proof.
+  intros H.
+  induction v;
+  inversion H;
+  inversion 1.
+Qed.
+
+Lemma value__result v : value v -> result v.
+Proof.
+  intros H.
+  apply value__ind;
+  intros;
+  auto using result, value__is_error.
+Qed.
+
+Lemma result__value v : result v -> ~ is_error v-> value v.
+Admitted.
 
 Lemma is_error_dec t : {is_error t} + {~ is_error t}.
 Proof.
@@ -87,10 +156,10 @@ induction H.
   left. auto.
 Defined.
 
-Lemma value_dec t : {value t} + {~ value t}.
+Lemma result_dec t : {result t} + {~ result t}.
 Proof.
   apply term__rect with
-    (P := fun t => {value t} + {~value t})
+    (P := fun t => {result t} + {~result t})
     (Q := fun b => unit).
   all: intros.
   all: try solve
@@ -118,16 +187,17 @@ Definition is_error_beq (t : term) : bool :=
     | _       => false
   end.
 
-Fixpoint value_beq (t : term) :=
+Fixpoint result_beq (t : term) :=
   match t with
     | LamAbs x T t0 => true
     | TyAbs X K t   => true
-    | IWrap F T v   => value_beq v && negb (is_error_beq v)
+    | IWrap F T v   => result_beq v && negb (is_error_beq v)
     | Constant u    => true
     | Error T       => true
     | _ => false
   end
   .
 
-Lemma dec_value_value : forall t, value_beq t = true -> value t.
+Lemma dec_result_result : forall t, result_beq t = true -> result t.
 Admitted.
+
