src/PlutusIR/Semantics/Dynamic/Bigstep/EvalValue.v
@@ -4,10 +4,10 @@ Require Import PlutusCert.PlutusIR.Semantics.Dynamic.Bigstep.
 
 Require Import Lia.
 
-Lemma eval_value :
-  forall v, value v -> v =[0]=> v.
+Lemma eval_result :
+  forall v, result v -> v =[0]=> v.
 Proof with (autounfold; (eauto || (try lia))).
-  apply value__ind.
+  apply result__ind.
   all: intros.
   all: try solve [constructor; eauto].
   (* Constr*)
@@ -17,7 +17,7 @@ Proof with (autounfold; (eauto || (try lia))).
       eapply E_Constr_cons with (k_t := 0) (k_ts := 0)...
 Qed.
 
-Corollary eval_value__value : forall v,
-    value v ->
+Corollary eval_result__result : forall v,
+    result v ->
     v =[0]=> v.
-Proof. apply eval_value. Qed.
+Proof. apply eval_result. Qed.
